3rd version

prototype/unstacked_borrows_pseudo.dfy
@@ -1,225 +1,317 @@
 datatype Tag = Unique(t: nat, c: nat) | SharedRO(t: nat, c:nat) | SharedRW(t: nat, c: nat) 
-              | SharedRWBot | Disabled
+              | Disabled | Unknown
 
 class State {
    var counter: nat; // used to generate new id
    var mem: array<int>;
    var tagmem: array<Tag>;
-   var ancestors: map<Tag, set<Tag>>;
-   var predecessor: map<Tag, Tag>;
-   // indicate if ShareRW(Bot) is on stack
-   var raw: array<bool>;   
-   // record the last SharedRO(t, c)
-   var lastread: array<Tag>;
+   
+   // the tag from which a rawfrom ponter bprrow
+   var rawfrom: array<int>;  
+
+   constructor(mem: array<int>)
+   ensures fresh(tagmem) && fresh(rawfrom);
+   ensures this.mem == mem && counter == 0;
+   ensures forall i:: 0 <= i && i < tagmem.Length ==> tagmem[i] == Unknown;
+   ensures forall i:: 0 <= i && i < rawfrom.Length ==> rawfrom[i] == -1;
+   ensures valid();
+   {
+     this.mem := mem;
+     tagmem := new Tag[mem.Length](_ => Unknown);
+     rawfrom := new int[mem.Length](_ => -1);
+     counter := 0;
+     
+   }
+
+   predicate valid()
+   reads this, mem, tagmem, rawfrom;
+   {
+    mem.Length == tagmem.Length && mem.Length == rawfrom.Length 
+   } 
+
+   predicate valid_addr(addr: int)
+   requires valid();
+   reads this, mem,tagmem, rawfrom;
+   {
+      0 <= addr && addr < mem.Length
+   }
+
+predicate invalidTag(addr: nat, tag: Tag)
+ requires valid() && valid_addr(addr);
+ reads this, tagmem, rawfrom, mem;
+ {
+    match (tagmem[addr], tag)
+    case (Unique(n1, c1), Unique(n2, c2)) => 
+     if (rawfrom[addr] != -1) then n2 != n1 
+      else n1 < n2
+    case (SharedRO(n1, c1), Unique(n2, c2)) => n1 < n2
+    case (Unique(n1, c1), SharedRO(n2, c2)) => n2 <= n2
+    case (SharedRW(n1, c1), SharedRO(n2, c2)) => n2 <= n2
+    case (SharedRO(n1, c1), SharedRO(n2, c2)) => false
+    case (Unknown, _) => false
+    case (_, _) => true
+}  
+
+predicate validTag(addr: nat, tag: Tag)
+requires valid() && valid_addr(addr);
+reads this, tagmem, rawfrom, mem;
+{
+  
+   tagmem[addr] == Unknown 
+   ||  
+   (tagmem[addr] != Unknown ==> !invalidTag(addr, tag))
+}
+    
    
    method generateID() returns (ret: nat) 
+   requires valid();
    modifies this;
+   ensures counter == old(counter) + 1 && ret == counter;
+   ensures mem == old(mem) && tagmem == old(tagmem) && rawfrom == old(rawfrom);
+   ensures forall i :: 0 <= i && i < tagmem.Length  ==> tagmem[i] == old(tagmem[i]);
+   ensures forall i :: 0 <= i && i < rawfrom.Length  ==> rawfrom[i] == old(rawfrom[i]);
+   ensures valid();
    {
      counter := counter + 1;
      ret := counter;
    }
    
    predicate isWritable(p: Pointer)
+   requires valid();
    requires p.valid(this);
-   reads this, p;
+   reads this, mem, rawfrom, tagmem, p;
    { 
       match p.tag
-      case Unique(t, c)  => p.tag in ancestors[tagmem[p.addr]]
-      case SharedRW(t, c) =>  p.tag in ancestors[tagmem[p.addr]]
+      case Unique(t, c)  => true
+      case SharedRW(t, c) =>  true
       case _ => false
    }
    
-   method write(p: Pointer, v: int)
+  method write(p: Pointer, v: int)
+     requires valid();
      requires p.valid(this) && isWritable(p);
-     modifies mem, tagmem;
+     modifies mem, tagmem, rawfrom;
+     ensures forall i :: 0 <= i && i < tagmem.Length && i != p.addr ==> tagmem[i] == old(tagmem[i]);
+     ensures forall i :: 0 <= i && i < mem.Length && i != p.addr ==> mem[i] == old(mem[i]);
+     ensures forall i :: 0 <= i && i < rawfrom.Length && i != p.addr ==> rawfrom[i] == old(rawfrom[i]);
+     ensures p.tag.Unique? ==> tagmem[p.addr] == p.tag;
+     ensures mem[p.addr] == v;
+     ensures valid();
    {
      match p.tag
      case Unique(t, c) =>
-       use1(p);
        mem[p.addr] := v;
+       tagmem[p.addr] := p.tag;
      case SharedRW(t, c) =>
         tagmem[p.addr] := p.tag; // update the top
          mem[p.addr] := v;
    }
    
- method use1(p: Pointer) 
- requires p.valid(this);
-{
-  match p.tag
-  case Unique(t, c) =>  
-    // Rule (USE -1 ) 
-    // requires Unique(t) is in the stack
-    // p becomes the top
-    tagmem[p.addr] := p.tag; 
-}
-
-method use2(p: Pointer)
-requires p.valid(this);
-{
-  if (raw[p.addr]) { // Pointer(l, Bot)
-    // pop up anything above SharedRWBot
-    tagmem[p.addr] := SharedRWBot;
-  } else{
-    match p.tag
-    case Unique(t, c) => // Pointer(l, t)
-    // pop up anything above Pointer(l, t)
-    tagmem[p.addr] := p.tag;
-  }
-}
-   
    method read(p: Pointer) returns (r: int)
+   requires valid();
    requires p.valid(this);
+   modifies tagmem;
+   ensures forall i :: 0 <= i && i < tagmem.Length && i != p.addr ==> tagmem[i] == old(tagmem[i]);
+   ensures forall i :: 0 <= i && i < mem.Length && i != p.addr ==> mem[i] == old(mem[i]);
+   ensures forall i :: 0 <= i && i < rawfrom.Length && i != p.addr ==> rawfrom[i] == old(rawfrom[i]);
+   ensures p.tag.Unique? ==> tagmem[p.addr] == p.tag;
+   ensures valid();
    {
      r := mem[p.addr];
      match p.tag
      case Unique(t, c) =>
-        use1(p);
+        tagmem[p.addr] := p.tag;
      case SharedRO(t, c) =>
       // nothing to do
      case SharedRW(t, c) => 
       // ?
-     
+     case _ => // ?
    }
 } 
+   
+
    
 
 class Pointer{
   var addr: nat;
   var tag: Tag;
   
- predicate valid(s: State){
-    tag in s.ancestors[s.tagmem[addr]]
-  }
-  
-  constructor(addr: nat, tag: Tag) {
+ predicate valid(s: State)
+ requires s.valid();
+ reads s, s.tagmem, s.rawfrom, s.mem, this;
+ {
+    s.valid_addr(addr) && s.validTag(addr, tag)
+ }
+ 
+ constructor(addr: nat, tag: Tag, s: State) 
+  requires s.valid() && s.valid_addr(addr);
+  requires s.validTag(addr, tag);
+  ensures this.addr == addr && this.tag == tag;
+  ensures valid(s);
+  {
     this.addr := addr;
     this.tag := tag;
   }
 }
 
-method createOwner(addr: nat, s: State)  returns(ret: Pointer) 
-modifies s;
-{
-   var newID := s.generateID();
-   var new_tag := Unique(newID, 1);
-   ret := new Pointer(addr, new_tag);
-   s.ancestors := s.ancestors[new_tag := {new_tag}];
-   s.predecessor := s.predecessor[new_tag := new_tag];
-   s.raw[addr] := false;
-}
-
 method createMutableRef(p: Pointer, s: State) returns(ret: Pointer)
-requires p.valid(s);
-modifies s;
+requires s.valid() &&  s.valid_addr(p.addr) /* p.valid(s) */ && p.tag.Unique?;
+modifies s, s.tagmem, s.rawfrom;
+ensures s.tagmem == old(s.tagmem) && s.mem == old(s.mem) && s.rawfrom == old(s.rawfrom);
+ensures s.counter == old(s.counter) + 1;
+ensures forall i :: 0 <= i && i < s.tagmem.Length && i != p.addr ==> s.tagmem[i] == old(s.tagmem[i]);
+ensures forall i :: 0 <= i && i < s.rawfrom.Length && i != p.addr ==> s.rawfrom[i] == old(s.rawfrom[i]);
+ensures s.tagmem[p.addr] == ret.tag && s.rawfrom[p.addr] == -1;
+ensures ret.addr == p.addr && ret.tag == Unique(s.counter, p.tag.c);
+ensures fresh(ret);
+ensures s.valid() && ret.valid(s);
+// ensures s.valid() && p.valid(s);
 {
   var newID := s.generateID();
   
-  var predecessor_of_top := s.predecessor[p.tag];
-  var ancestors_of_top := s.ancestors[p.tag];
-  
   match p.tag
-    case Unique(t, c) =>
-        /*
-            let x = & mut p;
-            1. it is considered as a use of p
-            2. generate a fresh tag for the new reference x, i.e., Unique(t', c)
-            3. record Unique(t', c)'s predecessor
-            4. record Unique(t',c)'s ancestors
-            5. push Unique(t', c) to the stack
-        */
-       var top := s.tagmem[p.addr];
-       var newtag := Unique(newID, c);
-       s.use1(p);
-       ret := new Pointer(p.addr, newtag);
-       s.predecessor := s.predecessor[newtag := predecessor_of_top];
-       s.ancestors := s.ancestors[newtag := ancestors_of_top + {newtag}];
+    case Unique(t, c?) =>
+       var newtag := Unique(newID, c?);
        s.tagmem[p.addr] := newtag;
-    case Raw =>
+       s.rawfrom[p.addr] := -1;
+       ret := new Pointer(p.addr, newtag, s);
+   // case _ =>
+   //    ret := new Pointer(p.addr, Disabled, s);
        // todo
 }
 
 /*
-Rule (NEW-SHARE-REF-1)
-*/
-method createShareRef(p: Pointer, s: State) returns(ret: Pointer)
-requires p.valid(s);
-modifies s;
-{
-  var newID := s.generateID();
-  var predecessor_of_top := s.predecessor[p.tag];
-  var ancestors_of_top := s.ancestors[p.tag];
-  
-  /*
-  1. consider a read access to p
-  2. generate a fresh tag for the new reference x, i.e., SharedRO(t', c)
-  3. record SharedRO(t', c)'s predecessor
-  4. record SharedRO(t', c)'s ancestors
-  5. update lastread as SharedRO(t', c)
-  6. push SharedRO(t', c) to the stack
-  */
-  readPointer(p, s);
-  var newtag := SharedRO(newID, 1);
-  ret := new Pointer(p.addr, newtag);
-  s.predecessor := s.predecessor[newtag := predecessor_of_top];
-  s.ancestors := s.ancestors[newtag := ancestors_of_top + {newtag}];
-  s.lastread[p.addr] := newtag;
-  s.tagmem[p.addr] := newtag;
-}
-
-// Rule READ-1
-// p could be Unique(t, c), SharedRO(t, c), SharedRW(t, c)
-method readPointer(p: Pointer, s: State)
-requires p.valid(s) ;
-modifies s, s.tagmem;
-{
-  // pop items off the stack until all the items above the item 
-  // with tag t are SharedRO(t, c)
-  s.tagmem[p.addr] := s.lastread[p.addr];
-}
-
-/*
-Raw pointers can only be created from Unique(t)
+rawfrom pointers can only be created from Unique(t)
 let raw_pointer = &mut p as *mut i32;
 */
 method createMutableRawRef(p: Pointer, s: State) returns(ret: Pointer)
-requires p.valid(s);
-modifies s;
+requires s.valid() && s.valid_addr(p.addr);
+requires s.rawfrom[p.addr] == -1 ==> p.tag.Unique?;
+requires s.rawfrom[p.addr] != -1 ==> p.tag.Unique? && s.rawfrom[p.addr] == p.tag.t;
+modifies s, s.tagmem, s.rawfrom;
+ensures s.tagmem == old(s.tagmem) && s.mem == old(s.mem) && s.rawfrom == old(s.rawfrom);
+ensures s.counter == old(s.counter) + 1;
+ensures forall i :: 0 <= i && i < s.tagmem.Length && i != p.addr ==> s.tagmem[i] == old(s.tagmem[i]);
+ensures forall i :: 0 <= i && i < s.rawfrom.Length && i != p.addr ==> s.rawfrom[i] == old(s.rawfrom[i]);
+ensures p.tag.Unique? ==> s.tagmem[p.addr] == ret.tag && s.rawfrom[p.addr] == p.tag.t;
+ensures p.tag.Unique? ==> ret.addr == p.addr && ret.tag == Unique(s.counter, p.tag.c);
+ensures fresh(ret);
+ensures s.valid() && ret.valid(s);
 {
   var newID := s.generateID();
-  var top := s.tagmem[p.addr];
-  var predecessor_of_top := s.predecessor[p.tag];
-  var ancestors_of_top := s.ancestors[p.tag];
   
   match p.tag
-  case ShareRWBot =>
-      /*
-      1. a use of p
-      2. generate new pointer
-      3. record new tag's predecessor
-      4. record new tag's ancestors
-      5. push ShareRW(BOT) on the top
-      */
-      var newtag := Unique(newID, 1);
-      s.use2(p);
-      var ret := new Pointer(p.addr, newtag);
-      s.predecessor := s.predecessor[newtag := top];
-      s.ancestors := s.ancestors[newtag := s.ancestors[top] + {newtag}];
+  case Unique(t, c?) =>
+      var newtag := Unique(newID, c?);
       s.tagmem[p.addr] := newtag;
-   case Unique(t, c) =>
-      /*
-      Rule (NEW-MUTABLE-RAW-1)
-      1. a use of p (USE-2)
-      2. generate new pointer
-      3. record new tag's predecessor
-      4. record new tag's ancestors
-      5. push ShareRW(BOT) on the top
-      6. mark the addr as raw
-      */
-      var newtag := SharedRWBot;
-      s.use2(p);
-      var ret := new Pointer(p.addr, newtag);
-      s.predecessor := s.predecessor[newtag := predecessor_of_top];
-      s.ancestors := s.ancestors[newtag := ancestors_of_top + {newtag}];
-      s.tagmem[p.addr] := newtag;
-      s.raw[p.addr] := true;
+      s.rawfrom[p.addr] := t;
+      ret := new Pointer(p.addr, newtag, s);
+      assert ret.tag.t == s.tagmem[p.addr].t;
+//  case Unique(t, c) =>
+//      var newtag := SharedRWBot;
+//      var ret := new Pointer(p.addr, newtag, s);
+//      s.tagmem[p.addr] := newtag;
+//      s.rawfrom[p.addr] := true;
+}
+
+
+/*
+Rule (NEW-SHARE-REF-1)
+*/
+method createSharedRO(p: Pointer, s: State) returns(ret: Pointer)
+requires s.valid() && s.valid_addr(p.addr);
+requires p.tag.Unique? || p.tag.SharedRO?;
+modifies s, s.tagmem, s.rawfrom;
+ensures s.tagmem == old(s.tagmem) && s.mem == old(s.mem) && s.rawfrom == old(s.rawfrom);
+ensures s.counter == old(s.counter) + 1;
+ensures forall i :: 0 <= i && i < s.tagmem.Length && i != p.addr ==> s.tagmem[i] == old(s.tagmem[i]);
+ensures forall i :: 0 <= i && i < s.rawfrom.Length  ==> s.rawfrom[i] == old(s.rawfrom[i]);
+ensures ret.addr == p.addr && ret.tag == SharedRO(s.counter, p.tag.c);
+ensures fresh(ret);
+ensures s.valid() && ret.valid(s);
+{
+  var newID := s.generateID();
+  var newtag := SharedRO(newID, p.tag.c);
+  match p.tag
+  case Unique(t, c?) =>
+    s.tagmem[p.addr] := newtag;
+    ret := new Pointer(p.addr, newtag, s);
+  case SharedRO(t, c?) =>
+    s.tagmem[p.addr] := newtag;
+    ret := new Pointer(p.addr, newtag, s);
+}
+
+// This client follows stack principle
+method mutableTest(mem:array<int>)
+  modifies mem;
+{
+  var s := new State(mem);
+      
+  // let mut local1 = 5;
+  var local1: nat;
+  var tag1 := s.generateID();
+  if(0 < local1 < mem.Length){
+    assert s.tagmem[local1] == Unknown;
+    mem[local1] := 5;
+    assert s.tagmem[local1] == Unknown;
+    var ref1: Pointer := new Pointer(local1, Unique(tag1, 1), s);
+  
+    var ref2: Pointer := createMutableRef(ref1, s);
+    
+    assert(ref2.valid(s));
+  
+    // function call starts
+    s.write(ref1, 42);
+   // s.write(ref2, 13);
+    assert !ref2.valid(s);
+  }
+}
+
+
+method mutableRawTest(mem:array<int>)
+  modifies mem;
+{
+    var s := new State(mem);
+        
+    // let mut local1 = 5;
+    var local1: nat;
+    var tag1 := s.generateID();
+    if(0 < local1 < mem.Length){
+      mem[local1] := 5;
+      var ref1: Pointer := new Pointer(local1, Unique(tag1, 1), s);
+     // s.write(ref1, 42);
+      var ref2: Pointer := createMutableRawRef(ref1, s);
+      
+      assert(ref2.valid(s));
+      var ref3: Pointer := createMutableRawRef(ref1, s);
+      assert(ref3.valid(s));
+      var ref4: Pointer := createMutableRawRef(ref1, s);
+      assert(!ref3.valid(s));
+    }
+
+  }
+
+method mutableSharedROTest(mem:array<int>)
+modifies mem;
+{
+  var s := new State(mem);
+        
+  // let mut local1 = 5;
+  var local1: nat;
+  var tag1 := s.generateID();
+  if(0 < local1 < mem.Length){
+      mem[local1] := 5;
+      var ref1: Pointer := new Pointer(local1, Unique(tag1, 1), s);
+     // s.write(ref1, 42);
+      var ref2: Pointer := createMutableRef(ref1, s);
+      
+      assert(ref2.valid(s));
+      var ref3: Pointer := createSharedRO(ref2, s);
+      assert(ref3.valid(s));
+      var ref4: Pointer := createSharedRO(ref2, s);
+      assert(ref4.valid(s));
+      var ref5: Pointer := createMutableRef(ref2, s);
+      assert(!ref4.valid(s));
+
+  }
 }
